README.md
@@ -1,36 +1,15 @@
 # LTS-formalization
-Formalization of LTS, Datalog, PDS and more
+This repository contains a number of formalizations based on labelled transition systems.
 
 ## Datalog
-Notes in Datalog folder
+The Datalog subfolder contains a formalization of Datalog programs for program analysis.
+
 
 ## PDS
-Notes in PDS folder and here:
+The PDS subfolder contains a formalization of reachability for pushdown systems.
 
-Formalization of push down systems
-
-PDS.thy is a new version where using locales and libraries
-
-morten_* are Morten's original version 
-anders_* are the same as Morten's with some additions
-
-
+Paper: https://www21.in.tum.de/~traytel/papers/fmcad22-pds/pds.pdf
 Based on this thesis: http://www.lsv.fr/Publis/PAPERS/PDF/schwoon-phd02.pdf
 
-
-Future work:
-https://github.com/DEIS-Tools/PDAAAL/blob/master/src/pdaaal/Solver.h#L92
-
-
-LTS formalizations:
-	https://www.isa-afp.org/entries/Transition_Systems_and_Automata.html
-	Not a good fit, because LTS are defined differently
-
-	afp-2021/thys/CAVA_LTL_Modelchecker/SM/Lib/LTS.thy
-	Similar to what we are doing, but very small.
-
-	There is a comprehensive overview of Graph and LTS libraries:
-	https://github.com/wimmers/archive-of-graph-formalizations
-
-	See also Anders's mail to Simon "Formalizing model checking"
-
+## WPDS
+A work in progress formalization of reachability for weighted pushdown systems.
