attic/README.txt
@@ -1,2 +1,10 @@
-Some old versions
+This folder contains Some old versions.
 
+Here are some old notes:
+
+morten_* are Morten's original version 
+anders_* are the same as Morten's with some additions
+
+
+Future work:
+https://github.com/DEIS-Tools/PDAAAL/blob/master/src/pdaaal/Solver.h#L92
